progs/verif_message.v
@@ -715,13 +715,6 @@ repeat flatten_sepcon_in_SEP.
 focus_SEP 3 1.
 get_global_function' _intpair_deserialize.
 get_global_function' _intpair_serialize.
-apply semax_seq with FF; [ | apply semax_ff].
-replace (overridePost FF POSTCONDITION) with POSTCONDITION
- by (unfold POSTCONDITION, abbreviate;
-      extensionality ek vl rho;
-      unfold overridePost, frame_ret_assert, function_body_ret_assert;
-      destruct ek; simpl; auto; normalize;
-      apply pred_ext; simpl; normalize).
 eapply semax_pre.
 frame_SEP' (0::nil).
 unfold main_pre, globvars2pred, prog_vars. simpl map.
